compiler/backend/word_cseScript.sml
@@ -1,6 +1,8 @@
 open Parse preamble wordLangTheory asmTheory sptreeTheory listTheory
      pred_setTheory;
 
+open jsonLangTheory presLangTheory;
+
 val _ = new_theory "word_cse";
 
 val _ = monadsyntax.temp_add_monadsyntax();
@@ -10,13 +12,23 @@ val _ = overload_on("monad_bind",``OPTION_BIND``);
 val _ = Datatype `
   vnumber = VConst ('a word)
           | VN num`;
-
 (*
  * Supported operations, used as labels on graph nodes.
  * Non-deterministic operations are marked as unknown
  *)
 val _ = Datatype `
+  wideop = High
+         | Low`
+
+val _ = Datatype `
   vop = VOp binop
+      | VShift shift num
+      | VDiv
+      | VLongMul wideop
+      | VLongDiv wideop
+      | VAddCarry wideop
+      | VAddOverflow wideop
+      | VSubOverflow wideop
       | VUnknown`;
 
 (*
@@ -30,6 +42,7 @@ val _ = Datatype `
              uses : unit spt ;
              held : unit spt |>`;
 
+
 (*
  * Numbering state.
  * Holds the next value number and all nodes.
@@ -39,6 +52,24 @@ val _ = Datatype `
   vnumbering = <| vnums : ('a vnumber) spt ;
                   vnodes : ('a vnode) spt ;
                   next : num |>`;
+
+val _ = Datatype `
+  event = RedunMove
+        | Merge
+        | Init
+        | Unassign
+        | Assign 
+        | RedunOp ('a prog)`;
+
+val log_event_def = Define `
+  (log_event RedunMove = empty_ffi (strlit "redun move")) ∧
+  (log_event Merge = empty_ffi (strlit "merge")) ∧
+  (log_event Init = empty_ffi (strlit "init")) ∧
+  (log_event Assign = empty_ffi (strlit "assign")) ∧
+  (log_event Unassign = empty_ffi (strlit "unassign")) ∧
+  (log_event (RedunOp Skip) = empty_ffi (strlit "redun skip")) ∧
+  (log_event (RedunOp (Inst _)) = empty_ffi (strlit "redun const")) ∧
+  (log_event (RedunOp (Move _ _)) = empty_ffi (strlit "redun copy"))`;
 
 val initial_vn_def = Define `
   initial_vn = <| vnums := LN ; vnodes := LN ; next := 0 |>`;
@@ -70,19 +101,25 @@ val get_nums_def = Define `
   get_nums vars nums = MAP (\v. get_num v nums) vars`;
 
 val unassign_num_def = Define `
-  unassign_num var nums =
+  unassign_num var (nums :'a vnumbering) =
     case get_num var nums of
       | SOME (VN v) =>
+          let _ = log_event (Unassign :'a event) in
           nums with <| vnums updated_by (delete var) ;
                        vnodes updated_by (delete_held var v) |>
-      | _ => nums with vnums updated_by (delete var)`;
+      | SOME (VConst w) =>
+          let _ = log_event (Unassign :'a event) in
+          nums with vnums updated_by (delete var)
+      | NONE => nums`;
 
 val assign_num_def = Define `
-  (assign_num var (VN v) nums =
+  (assign_num var (VN v) (nums :'a vnumbering) =
+    let _ = log_event (Assign :'a event) in
     (unassign_num var nums) with
       <| vnums updated_by (insert var (VN v)) ;
          vnodes updated_by (insert_held var v) |>) ∧
   (assign_num var (VConst w) nums =
+    let _ = log_event (Assign :'a event) in
     (unassign_num var nums) with
       vnums updated_by (insert var (VConst w)))`;
 
@@ -104,12 +141,13 @@ val get_moves_def = Define `
 
 val redun_move_def = Define `
   (redun_move [] acc nums = acc) ∧
-  (redun_move ((dst, src)::xs) acc nums = 
+  (redun_move ((dst, src)::xs) acc (nums : 'a vnumbering) = 
     let
       vn1 = get_num dst nums;
       vn2 = get_num src nums
     in
-      if IS_SOME(vn1) ∧ vn1 = vn2 then redun_move xs acc nums
+      if IS_SOME(vn1) ∧ vn1 = vn2 then
+        (let _ = (log_event (RedunMove : 'a event)) in redun_move xs acc nums)
       else redun_move xs ((dst,src)::acc) nums)`;
 
 val cse_move_def = Define `
@@ -137,6 +175,34 @@ val all_const_def = Define `
  *)
 val fold_def = Define `
   (fold (VOp op) ws = word_op op ws) ∧
+  (fold (VShift sh n) [w] = word_sh sh w n) ∧
+  (fold VDiv [w1; w2] = if w2 ≠ 0w then SOME(w1 / w2) else NONE) ∧
+  (fold (VLongMul wide) [w1; w2] =
+    let r = w2n w1 * w2n w2 in
+    case wide of
+      | High => SOME (n2w (r DIV dimword(:'a)))
+      | Low => SOME (n2w r)) ∧
+  (fold (VLongDiv wide) [w1; w2; w3] =
+    let n = w2n w1 * dimword (:'a) + w2n w2 in
+    let d = w2n w3 in
+    let q = n DIV d in
+    if (d = 0 ∨ q >= dimword(:'a)) then NONE else
+      case wide of
+        | High => SOME (n2w (n MOD d))
+        | Low => SOME (n2w q)) ∧
+  (fold (VAddCarry wide) [w1; w2; w3] =
+    let res = w2n w1 + w2n w2 + if w3 = 0w then 0 else 1 in
+      case wide of
+        | High => SOME (n2w res)
+        | Low => SOME (if dimword(:'a) ≤ res then (1w:'a word) else 0w)) ∧
+  (fold (VAddOverflow wide) [w1; w2] =
+    case wide of
+      | High => SOME (w1 + w2)
+      | Low => SOME (if w2i (w1 + w2) ≠ w2i w1 + w2i w2 then 1w else 0w)) ∧
+  (fold (VSubOverflow wide) [w1; w2] =
+    case wide of
+      | High => SOME (w1 - w2)
+      | Low => SOME (if w2i (w1 - w2) ≠ w2i w1 - w2i w2 then 1w else 0w)) ∧
   (fold label ws = NONE)`;
 
 val attempt_fold_def = Define `
@@ -188,20 +254,45 @@ val find_exp_def = Define `
 (*
  * Generate either a move, const or skip depending on the situation
  *)
-val gen_move_def = Define `
-  (gen_move dst ((VN n) : α vnumber) (nums : α vnumbering) =
+val pick_source_def = Define `
+  pick_source n nums =
     case lookup n nums.vnodes of
       | SOME node =>
           (case toAList node.held of
-            | ((i,p)::t) => SOME (Move 0 [(dst,i)])
+            | ((i,p)::t) => SOME i
             | _ => NONE)
+      | NONE => NONE`;
+
+val gen_move_def = Define `
+  (gen_move dst ((VN n) : α vnumber) (nums : α vnumbering) =
+    case pick_source n nums of
+      | SOME i => SOME (Move 0 [(dst,i)])
       | NONE => NONE) ∧
   (gen_move dst (VConst w) nums = SOME (Inst (Const dst w)))`;
+
+val gen_wide_move_def = Define `
+  (gen_wide_move dst1 dst2 (VN n1) (VN n2) nums =
+    case (pick_source n1 nums, pick_source n2 nums) of
+      | SOME i1, SOME i2 => SOME (Move 0 [(dst1,i1);(dst2,i2)])
+      | _, _ => NONE) ∧
+  (gen_wide_move dst1 dst2 (VConst c) (VN n) nums =
+    case (gen_move dst2 (VN n) nums, gen_move dst1 (VConst c) nums) of
+      | SOME p1, SOME p2 => SOME (Seq p1 p2)
+      | _, _ => NONE) ∧
+  (gen_wide_move dst1 dst2 vn1 vn2 nums =
+    case (gen_move dst1 vn1 nums, gen_move dst2 vn2 nums) of
+      | SOME p1, SOME p2 => SOME (Seq p1 p2)
+      | _, _ => NONE)`;
 
 val gen_prog_def = Define `
   gen_prog dst vn nums =
     if get_num dst nums = SOME vn then SOME (Skip)
     else gen_move dst vn nums`;
+
+val gen_wide_prog_def = Define `
+  gen_wide_prog dst1 dst2 vn1 vn2 nums =
+    if dst1 = dst2 then gen_prog dst2 vn2 nums
+    else gen_wide_move dst1 dst2 vn1 vn2 nums`;
 
 (* Attempt to match/fold the expression and generate a replacement prog *)
 val redun_exp_def = Define `
@@ -209,7 +300,18 @@ val redun_exp_def = Define `
     do
       vn <- find_exp label vns nums;
       prog <- gen_prog dst vn nums;
+      _ <- SOME (log_event (RedunOp prog));
       SOME (prog, assign_num dst vn nums)
+    od`;
+
+val redun_wide_exp_def = Define `
+  redun_wide_exp lbl dst1 dst2 vns nums =
+    do
+      vn1 <- find_exp (lbl High) vns nums;
+      vn2 <- find_exp (lbl Low) vns nums;
+      prog <- gen_wide_prog dst1 dst2 vn1 vn2 nums;
+      _ <- SOME (log_event (RedunOp prog));
+      SOME (prog, assign_num dst2 vn2 (assign_num dst1 vn1 nums))
     od`;
 
 (*
@@ -235,145 +337,180 @@ val add_vnode_def = Define `
   add_vnode lbl var ops nums =
     assign_num var (VN nums.next) (add_empty_vnode lbl ops nums)`;
 
+val add_wide_vnode_def = Define `
+  add_wide_vnode lbl var1 var2 ops nums =
+    let
+      lbl1 = add_empty_vnode (lbl High) ops nums;
+      lbl2 = add_empty_vnode (lbl Low) ops lbl1;
+      l = [(var1, SOME (VN nums.next)); (var2, SOME (VN lbl1.next))]
+    in
+      assign_nums l lbl2`;
+
+(*
+ * Given a var, either find it in nums or create an Unknown VN to represent it
+ * Modified flag in the result represents whether any where created
+ *)
 val get_or_assign_num_def = Define `
   get_or_assign_num var nums =
     case get_num var nums of
-      | SOME vn => (vn, nums)
-      | NONE => (VN nums.next, add_vnode VUnknown var [] nums)`
+      | SOME vn => (vn,nums,F)
+      | NONE => (VN nums.next,add_vnode VUnknown var [] nums,T)`
 
 val get_or_assign_nums_def = Define `
   (get_or_assign_nums (v::vs) nums =
     let
-      (vn,nums1) = get_or_assign_num v nums;
-      (vns,nums2) = get_or_assign_nums vs nums1
+      (vn,nums1,m1) = get_or_assign_num v nums;
+      (vns,nums2,m2) = get_or_assign_nums vs nums1
     in 
-      (vn::vns,nums2)) ∧
-  (get_or_assign_nums [] nums = ([],nums))`;
+      (vn::vns,nums2,m1 ∨ m2)) ∧
+  (get_or_assign_nums [] nums = ([],nums,F))`;
 
-val cse_binop_def = Define `
-  cse_binop op r1 r2 ri nums =
+(*
+ * Functions that take an expression in lbl,dsts,args form and
+ * either matches it with another in nums to produce a new prog or
+ * inserts the new expression into the graph
+ *)
+val cse_exp_def = Define `
+  cse_exp lbl dst args nums =
+    let (vns,nnums,modified) = get_or_assign_nums args nums in
+    if modified then (NONE, add_vnode lbl dst vns nnums)
+    else case redun_exp lbl dst vns nnums of
+      | SOME (nprog,n) => (SOME nprog,n)
+      | NONE => (NONE, add_vnode lbl dst vns nnums)`;
+
+val cse_const_exp_def = Define `
+  cse_const_exp lbl dst args c nums =
     let
-      lbl = VOp op;
-      orig = Inst (Arith (Binop op r1 r2 ri));
-      (vns,nnums) = case ri of
-        | Reg r3 => get_or_assign_nums [r2; r3] nums
-        | Imm w => let (vn,n) = get_or_assign_nums [r2] nums in (vn ++ [VConst w], n)
+      (vns1,nnums,modified) = get_or_assign_nums args nums;
+      vns = (vns1 ++ [VConst c])
     in
-      case redun_exp lbl r1 vns nnums of
-        | SOME res => res
-        | NONE => (orig, add_vnode lbl r1 vns nnums)`;
+      if modified then (NONE, add_vnode lbl dst vns nnums)
+      else case redun_exp lbl dst vns nnums of
+        | SOME (nprog,n) => (SOME nprog,n)
+        | NONE => (NONE, add_vnode lbl dst vns nnums)`;
+
+val cse_wide_exp_def = Define `
+  cse_wide_exp (lbl:wideop -> vop) dst1 dst2 args nums =
+    let
+      (vns,nnums,modified) = get_or_assign_nums args nums;
+      fnums = add_wide_vnode lbl dst1 dst2 vns nnums
+    in
+      if modified then (NONE,fnums)
+      else case redun_wide_exp lbl dst1 dst2 vns nums of
+        | SOME (nprog,n) => (SOME nprog,n)
+        | NONE => (NONE,fnums)`;
+
 
 (*
  * arith instructions
  *)
 val cse_arith_def = Define `
-  (cse_arith (Binop bop r1 r2 ri) nums = cse_binop bop r1 r2 ri nums) /\
-  (cse_arith (Shift s r1 r2 n) nums =
-    (Inst (Arith (Shift s r1 r2 n)), unassign_num r1 nums)) /\
-  (cse_arith (Div r1 r2 r3) nums =
-    (Inst (Arith (Div r1 r2 r3)), unassign_num r1 nums)) /\
+  (cse_arith (Binop op r1 r2 (Reg r)) nums = cse_exp (VOp op) r1 [r2;r] nums) ∧
+  (cse_arith (Shift s r1 r2 n) nums = cse_exp (VShift s n) r1 [r2] nums) ∧
+  (cse_arith (Div r1 r2 r3) nums = cse_exp VDiv r1 [r2;r3] nums) ∧
+
+  (cse_arith (Binop op r1 r2 (Imm c)) nums =
+    cse_const_exp (VOp op) r1 [r2] c nums) ∧
+
   (cse_arith (LongMul r1 r2 r3 r4) nums =
-    (Inst (Arith (LongMul r1 r2 r3 r4)), unassign_num r2 (unassign_num r1 nums))) /\
+    cse_wide_exp VLongMul r1 r2 [r3;r4] nums) ∧
   (cse_arith (LongDiv r1 r2 r3 r4 r5) nums =
-    (Inst (Arith (LongDiv r1 r2 r3 r4 r5)), unassign_num r1 (unassign_num r2 nums))) /\
+    cse_wide_exp VLongDiv r2 r1 [r3;r4;r5] nums) ∧
   (cse_arith (AddCarry r1 r2 r3 r4) nums =
-    (Inst (Arith (AddCarry r1 r2 r3 r4)), unassign_num r4 (unassign_num r1 nums))) /\
+    cse_wide_exp VAddCarry r1 r4 [r2;r3;r4] nums) ∧
   (cse_arith (AddOverflow r1 r2 r3 r4) nums =
-    (Inst (Arith (AddOverflow r1 r2 r3 r4)), unassign_num r4 (unassign_num r1 nums))) /\
+    cse_wide_exp VAddOverflow r1 r4 [r2;r3] nums) ∧
   (cse_arith (SubOverflow r1 r2 r3 r4) nums =
-    (Inst (Arith (SubOverflow r1 r2 r3 r4)), unassign_num r4 (unassign_num r1 nums)))`;
+    cse_wide_exp VSubOverflow r1 r4 [r2;r3] nums)`;
 
 (*
  * floating point instructions
  *)
 val cse_fp_def = Define `
-  (cse_fp (FPLess r f1 f2) (nums : 'a vnumbering) =
-    (Inst (FP (FPLess r f1 f2)), unassign_num r nums)) ∧
-  (cse_fp (FPLessEqual r f1 f2) nums =
-    (Inst (FP (FPLessEqual r f1 f2)), unassign_num r nums)) ∧
-  (cse_fp (FPEqual r f1 f2) nums =
-    (Inst (FP (FPEqual r f1 f2)), unassign_num r nums)) ∧
+  (cse_fp (FPLess r f1 f2) nums = (NONE, unassign_num r nums)) ∧
+  (cse_fp (FPLessEqual r f1 f2) nums = (NONE, unassign_num r nums)) ∧
+  (cse_fp (FPEqual r f1 f2) nums = (NONE, unassign_num r nums)) ∧
   (cse_fp (FPMovToReg r1 r2 d) (nums : 'a vnumbering) =
-    (Inst (FP (FPMovToReg r1 r2 d)),
+    (NONE,
       if dimindex(:'a) = 64 then unassign_num r1 nums
       else unassign_num r2 (unassign_num r1 nums))) ∧
-  (cse_fp fp (nums :α vnumbering) = (Inst (FP fp) :α prog, nums))`;
+  (cse_fp fp (nums :α vnumbering) = (NONE :α prog option, nums))`;
 
 (*
  * memory instructions
  *)
 val cse_mem_def = Define `
-  (cse_mem Load r a nums = (Inst (Mem Load r a), unassign_num r nums)) /\
-  (cse_mem Load8 r a nums = (Inst (Mem Load8 r a), unassign_num r nums)) /\
-  (cse_mem memop r a (nums :α vnumbering) =
-    (Inst (Mem memop r a) :α prog, nums))`;
+  (cse_mem Load r a nums = (NONE, unassign_num r nums)) ∧
+  (cse_mem Load8 r a nums = (NONE, unassign_num r nums)) ∧
+  (cse_mem memop r a (nums :α vnumbering) = (NONE :α prog option, nums))`;
 
 val cse_inst_def = Define `
-  (cse_inst asm$Skip nums = (Inst (Skip), nums)) ∧
+  (cse_inst Skip nums = (Inst (asm$Skip), nums)) ∧
   (cse_inst (Const dst w) nums =
     (Inst (Const dst w), assign_num dst (VConst w) nums)) ∧
-  (cse_inst (Arith a) nums = cse_arith a nums) ∧
-  (cse_inst (FP fp) nums = cse_fp fp nums) ∧
-  (cse_inst (Mem memop r a) nums = cse_mem memop r a nums)`;
-
-(*
- * manage modifications to vnums due to assigns
- * there should be none after inst sel, so just maintain correctness
- *)
-val cse_assign_def = Define `
-  cse_assign dst exp (nums :α vnumbering) =
-    (wordLang$Assign dst exp :α prog, unassign_num dst nums)`;
-
-val cse_get_def = Define `
-  cse_get dst name (nums :α vnumbering) =
-    (Get dst name :α prog, unassign_num dst nums)`;
+  (cse_inst (Arith a) nums =
+    let (np,nnums) = cse_arith a nums in
+      ((case np of SOME p => p | NONE => Inst (Arith a)), nnums)) ∧
+  (cse_inst (FP fp) nums =
+    let (np,nnums) = cse_fp fp nums in
+      ((case np of SOME p => p | NONE => Inst (FP fp)), nnums)) ∧
+  (cse_inst (Mem memop r a) nums =
+    let (np,nnums) = cse_mem memop r a nums in
+      ((case np of SOME p => p | NONE => Inst (Mem memop r a)), nnums))`;
 
 (* logic for merging vnums at a join *)
 (* TODO: actually perform a merge of some sort *)
 (* TODO: Pruning of value graph *)
 val merge_vnums_def = Define `
   merge_vnums (vnums1 :α vnumbering) (vnums2 :α vnumbering) :α vnumbering =
-    initial_vn`;
+    let _ = log_event (Merge :α event) in initial_vn`;
 
 val cse_loop_def = Define `
   (* operations updating state *)
-  (cse_loop (Move pri moves) nums = cse_move pri moves nums) /\
-  (cse_loop (Assign dst exp) nums = cse_assign dst exp nums) /\
+  (cse_loop (Move pri moves) nums = cse_move pri moves nums) ∧
+  (cse_loop (Assign dst exp) nums = (Assign dst exp, unassign_num dst nums)) ∧
   (cse_loop (Inst i) nums = cse_inst i nums) ∧
-  (cse_loop (Get dst name) nums = cse_get dst name nums) /\
-  (cse_loop (LocValue dst n) nums = (LocValue dst n, unassign_num dst nums)) /\
+  (cse_loop (Get dst name) nums = (Get dst name, unassign_num dst nums)) ∧
+  (cse_loop (LocValue dst n) nums = (LocValue dst n, unassign_num dst nums)) ∧
+
   (* control flow *)
   (cse_loop (MustTerminate p) nums =
-    let (pn, numsn) = cse_loop p nums in
-      (MustTerminate pn, numsn)) /\
+    let (pn, numsn) = cse_loop p nums in (MustTerminate pn, numsn)) ∧
   (cse_loop (Seq p1 p2) nums =
     let
       (p1n, nums1) = cse_loop p1 nums;
       (p2n, nums2) = cse_loop p2 nums1
     in
-      (Seq p1n p2n, nums2)) /\
-  (* TODO: optimisations over comparisons *)
-  (cse_loop (wordLang$If cmp lhs rhs p1 p2) nums =
-    let (p1n, nums1) = cse_loop p1 nums in
-    let (p2n, nums2) = cse_loop p2 nums in
-    (wordLang$If cmp lhs rhs p1n p2n, merge_vnums nums1 nums2)) /\
+      (Seq p1n p2n, nums2)) ∧
+  (cse_loop (If cmp lhs rhs p1 p2) nums =
+    let
+      (p1n, nums1) = cse_loop p1 nums;
+      (p2n, nums2) = cse_loop p2 nums;
+    in
+      (If cmp lhs rhs p1n p2n, merge_vnums nums1 nums2)) ∧
+
   (* GC / Calls - reset nums *)
-  (cse_loop (Call ret dest args handler) nums =
+  (cse_loop (Call ret dest args handler) (nums : 'a vnumbering) =
+    let _ = log_event (Init : 'a event) in
     case ret of
       | NONE => (Call ret dest args handler, initial_vn)
       | SOME (n, names, ret_handler, l1, l2) =>
         (if handler = NONE then
            (let (ret_handlern, _) = cse_loop ret_handler initial_vn in
-           (Call (SOME (n, names, ret_handlern, l1, l2)) dest args handler, initial_vn))
+           (Call (SOME (n, names, ret_handlern, l1, l2)) dest args handler,
+             initial_vn))
          else
-           (Call ret dest args handler, initial_vn))) /\
-  (cse_loop (Alloc n names) nums = (Alloc n names, initial_vn)) /\
-  (cse_loop (FFI x0 x1 x2 x3 x4 names) nums = (FFI x0 x1 x2 x3 x4 names, initial_vn)) /\
+           (Call ret dest args handler, initial_vn))) ∧
+  (cse_loop (Alloc n names) (nums : 'a vnumbering) =
+    let _ = log_event (Init : 'a event) in (Alloc n names, initial_vn)) ∧
+  (cse_loop (FFI x0 x1 x2 x3 x4 names) (nums : 'a vnumbering) =
+    let _ = log_event (Init : 'a event) in (FFI x0 x1 x2 x3 x4 names, initial_vn)) ∧
+
   (* other instructions are ignored *)
-  (* TODO: potential opts for memory operations *)
-  (cse_loop (p : 'a prog) (nums : 'a vnumbering)  =  (p, nums))`;
+  (cse_loop (p :'a prog) (nums :'a vnumbering)  =  (p, nums))`;
 
 val cse_def = Define `
-  cse (p : 'a prog) = FST (cse_loop p (initial_vn : 'a vnumbering))`;
+  cse (p :'a prog) =
+    let _ = log_event (Init : 'a event) in FST (cse_loop p (initial_vn :'a vnumbering))`;
 
 val _ = export_theory();
